The chick has been slaughtered

src/rocq/Utils/StringUtil.v
@@ -1,6 +1,7 @@
-From Stdlib Require Import String Ascii List.
+From Stdlib Require Import Program String Ascii List Decimal ZArith.
 From Vellvm.Utils Require Import ListUtil.
 Import ListNotations.
+Open Scope string.
 
 Fixpoint string_fold_left {A} (f : A -> ascii -> A) (s:string) (acc:A) : A :=
   match s with
@@ -18,3 +19,162 @@ Definition string_of_list_ascii_tail_rec (s : list ascii) : string
 Definition list_ascii_of_string_tail_rec (s : string) : list ascii
   := rev_tail_rec (string_fold_left (fun acc ch => ch :: acc) s []).
 
+(* The following is reproduced from the QuickChick library to avoid a heavy dependency *)
+Section Show.
+
+  Fixpoint contents {A : Type} (s : A -> string) (l : list A) : string :=
+    match l with
+    | nil => ""%string
+    | cons h nil => s h
+    | cons h t => append (append (s h) "; ") (contents s t)
+    end.
+
+  Class Show (A : Type) : Type :=
+    { show : A -> string }.
+
+  Fixpoint show_uint (n : uint) : string :=
+    match n with
+    | Nil => ""
+    | D0 n => String "0" (show_uint n)
+    | D1 n => String "1" (show_uint n)
+    | D2 n => String "2" (show_uint n)
+    | D3 n => String "3" (show_uint n)
+    | D4 n => String "4" (show_uint n)
+    | D5 n => String "5" (show_uint n)
+    | D6 n => String "6" (show_uint n)
+    | D7 n => String "7" (show_uint n)
+    | D8 n => String "8" (show_uint n)
+    | D9 n => String "9" (show_uint n)
+    end.
+
+  Definition show_int (n : int) : string :=
+    match n with
+    | Pos n => show_uint n
+    | Neg n => String "-" (show_uint n)
+    end.
+
+  Definition show_nat (n : nat) : string :=
+    show_uint (Nat.to_uint n).
+
+  Definition show_bool (b : bool) : string :=
+    match b with
+    | true => "true"
+    | false => "false"
+    end.
+
+  Definition show_Z (n : Z) : string :=
+    show_int (Z.to_int n).
+
+  Definition show_N : N -> string :=
+    show_Z ∘ Z.of_N.
+
+  #[global] Instance showUint : Show uint :=
+    {|
+      show := show_uint
+    |}.
+
+  #[global] Instance showInt : Show int :=
+    {|
+      show := show_int
+    |}.
+
+  #[global] Instance showNat : Show nat :=
+    {|
+      show := show_nat
+    |}.
+
+  #[global] Instance showBool : Show bool :=
+    {|
+      show := show_bool
+    |}.
+
+  #[global] Instance showZ : Show Z :=
+    {|
+      show := show_Z
+    |}.
+
+  #[global] Instance showN : Show N :=
+    {|
+      show := show_N
+    |}.
+
+  Fixpoint from_list (s : list ascii) : string :=
+    match s with
+    | [] => EmptyString
+    | c :: s' => String c (from_list s')
+    end.
+
+  Definition unit_digit (n : nat) : ascii :=
+    ascii_of_nat ((n mod 10) + 48 (* 0 *)).
+
+  Definition three_digit (n : nat) : string :=
+    let n0 := unit_digit n in
+    let n1 := unit_digit (n / 10) in
+    let n2 := unit_digit (n / 100) in
+    from_list [n2; n1; n0].
+
+  Definition digit_of_ascii (c : ascii) : option nat :=
+    let n := nat_of_ascii c in
+    if ((48 <=? n)%nat && (n <=? 57)%nat)%bool then
+      Some (n - 48)
+    else
+      None.
+
+  Definition unthree_digit (c2 c1 c0 : ascii) : option ascii :=
+    let doa := digit_of_ascii in
+    match doa c2, doa c1, doa c0 with
+    | Some n2, Some n1, Some n0 =>
+        Some (ascii_of_nat (n2 * 100 + n1 * 10 + n0))
+    | _, _, _ => None
+    end.
+
+  Fixpoint show_quoted_string (s:string) : string :=
+    match s with
+    | EmptyString => """"
+    | String c s' =>
+        let quoted_s' := show_quoted_string s' in
+        let n := nat_of_ascii c in
+        if ascii_dec c "009" (* TAB *) then
+          "\t" ++ quoted_s'
+        else if ascii_dec c "010" (* NEWLINE *) then
+               "\n" ++ quoted_s'
+             else if ascii_dec c "013" (* CARRIAGE RETURN *) then
+                    "\r" ++ quoted_s'
+                  else if ascii_dec c """" (* DOUBLEQUOTE *) then
+                         "\""" ++ quoted_s'
+                       else if ascii_dec c "\" (* BACKSLASH *) then
+                              "\\" ++ quoted_s'
+                            else if ((n <? 32)%nat (* SPACE *)
+                                     || (126 <? n)%nat (* ~ *))%bool then
+                                   "\" ++ three_digit n ++ quoted_s'
+                                 else
+                                   String c quoted_s'
+    end.
+
+  #[global] Instance showString : Show string :=
+    {|
+      show s := String """" (show_quoted_string s)
+    |}.
+
+  
+  #[global] Instance showPair {A B : Type} `{_ : Show A} `{_ : Show B} : Show (A * B) :=
+    {|
+      show p := match p with (a,b) => ("(" ++ show a ++ ", " ++  show b ++ ")")%string end
+    |}.
+  
+  #[global] Instance showOpt {A : Type} `{_ : Show A} : Show (option A) :=
+    {|
+      show x := match x with
+                | Some x => "Some " ++ (show x)
+                | None => "None"
+                end
+    |}.
+
+  #[global] Instance showList {A : Type} `{_ : Show A} : Show (list A) :=
+    {|
+      show l := append "[" (append (contents show l) "]")
+    |}.
+
+  Definition newline := String "010" ""%string.
+  
+End Show.
